reduce cheats

examples/pkc_checker/array/scpog_arrayFullProgScript.sml
@@ -54,386 +54,6 @@ val b_inputLineTokens_specialize =
   |> Q.GEN `a` |> Q.ISPEC`SUM_TYPE STRING_TYPE INT`
   |> SIMP_RULE std_ss [blanks_v_thm,tokenize_v_thm,blanks_def] ;
 
-(*
-val parse_dimacs_body_arr = process_topdecs`
-  fun parse_dimacs_body_arr lno maxvar fd acc =
-  case TextIO.b_inputLineTokens #"\n" fd blanks tokenize of
-    None => Inr (List.rev acc)
-  | Some l =>
-    if nocomment_line l then
-      (case parse_clause maxvar l of
-        None => Inl (format_dimacs_failure lno "failed to parse line")
-      | Some cl => parse_dimacs_body_arr (lno+1) maxvar fd (cl::acc))
-    else parse_dimacs_body_arr (lno+1) maxvar fd acc` |> append_prog;
-
-Theorem parse_dimacs_body_arr_spec:
-  !lines fd fdv fs maxvar maxvarv acc accv lno lnov.
-  NUM lno lnov ∧
-  NUM maxvar maxvarv ∧
-  LIST_TYPE (LIST_TYPE INT) acc accv
-  ⇒
-  app (p : 'ffi ffi_proj)
-    ^(fetch_v "parse_dimacs_body_arr" (get_ml_prog_state()))
-    [lnov; maxvarv; fdv; accv]
-    (STDIO fs * INSTREAM_LINES #"\n" fd fdv lines fs)
-    (POSTv v.
-      & (∃err. SUM_TYPE STRING_TYPE (LIST_TYPE (LIST_TYPE INT))
-      (case parse_dimacs_body maxvar (FILTER nocomment_line (MAP toks lines)) acc of
-        NONE => INL err
-      | SOME x => INR x) v) *
-      SEP_EXISTS k lines'.
-         STDIO (forwardFD fs fd k) * INSTREAM_LINES #"\n" fd fdv lines' (forwardFD fs fd k))
-Proof
-  Induct
-  \\ simp []
-  \\ rpt strip_tac
-  \\ xcf "parse_dimacs_body_arr" (get_ml_prog_state ())
-  THEN1 (
-    xlet ‘(POSTv v.
-            SEP_EXISTS k.
-                STDIO (forwardFD fs fd k) *
-                INSTREAM_LINES #"\n" fd fdv [] (forwardFD fs fd k) *
-                &OPTION_TYPE (LIST_TYPE (SUM_TYPE STRING_TYPE INT)) NONE v)’
-    THEN1 (
-      xapp_spec b_inputLineTokens_specialize
-      \\ qexists_tac `emp`
-      \\ qexists_tac ‘[]’
-      \\ qexists_tac ‘fs’
-      \\ qexists_tac ‘fd’ \\ xsimpl \\ fs [])
-    \\ fs [std_preludeTheory.OPTION_TYPE_def] \\ rveq \\ fs []
-    \\ xmatch \\ fs []
-    \\ simp[parse_dimacs_body_def]
-    \\ xlet_autop
-    \\ xcon \\ xsimpl
-    \\ simp[SUM_TYPE_def]
-    \\ qexists_tac ‘k’ \\ xsimpl
-    \\ qexists_tac `[]` \\ xsimpl)
-  \\ xlet ‘(POSTv v.
-            SEP_EXISTS k.
-                STDIO (forwardFD fs fd k) *
-                INSTREAM_LINES #"\n" fd fdv lines (forwardFD fs fd k) *
-                & OPTION_TYPE (LIST_TYPE (SUM_TYPE STRING_TYPE INT)) (SOME (toks h)) v)’
-    THEN1 (
-      xapp_spec b_inputLineTokens_specialize
-      \\ qexists_tac `emp`
-      \\ qexists_tac ‘h::lines’
-      \\ qexists_tac ‘fs’
-      \\ qexists_tac ‘fd’ \\ xsimpl \\ fs []
-      \\ rw [] \\ qexists_tac ‘x’ \\ xsimpl
-      \\ simp[toks_def])
-  \\ fs [std_preludeTheory.OPTION_TYPE_def] \\ rveq \\ fs []
-  \\ xmatch \\ fs []
-  \\ xlet_autop
-  \\ reverse IF_CASES_TAC
-  >- (
-    xif >> asm_exists_tac>>xsimpl>>
-    xlet_autop>>
-    xapp>> xsimpl>>
-    asm_exists_tac>> simp[]>>
-    asm_exists_tac>> simp[]>>
-    qexists_tac`emp`>>xsimpl>>
-    qexists_tac`forwardFD fs fd k`>>
-    qexists_tac`fd`>>xsimpl>>
-    qexists_tac`acc`>>xsimpl>>
-    rw[]>>
-    qexists_tac`k+x`>>
-    simp[GSYM fsFFIPropsTheory.forwardFD_o]>>
-    qexists_tac`x'`>>xsimpl>>
-    metis_tac[])>>
-  xif>> asm_exists_tac>>simp[]>>
-  xlet_autop>>
-  simp[parse_dimacs_body_def]>>
-  Cases_on`parse_clause maxvar (toks h)`>>fs[OPTION_TYPE_def]
-  >- (
-    xmatch>>
-    xlet_autop>>
-    xcon>>
-    xsimpl>>
-    qexists_tac`k`>> qexists_tac`lines`>>xsimpl>>
-    simp[SUM_TYPE_def]>>
-    metis_tac[])>>
-  xmatch>>
-  xlet_autop>>
-  xlet_autop>>
-  xapp>>
-  xsimpl>>
-  asm_exists_tac>>simp[]>>
-  asm_exists_tac>>simp[]>>
-  qexists_tac`emp`>>
-  qexists_tac`forwardFD fs fd k`>>
-  qexists_tac`fd`>>
-  qexists_tac`x::acc`>>
-  xsimpl>>
-  simp[LIST_TYPE_def]>>rw[]>>
-  qexists_tac`k+x'`>>
-  qexists_tac`x''`>>
-  simp[GSYM fsFFIPropsTheory.forwardFD_o]>>
-  xsimpl>>
-  metis_tac[]
-QED
-
-val parse_dimacs_toks_arr = process_topdecs`
-  fun parse_dimacs_toks_arr lno fd =
-  case TextIO.b_inputLineTokens #"\n" fd blanks tokenize of
-    None => Inl (format_dimacs_failure lno "failed to find header")
-  | Some l =>
-    if nocomment_line l then
-      (case parse_header_line l of
-        None => Inl (format_dimacs_failure lno "failed to parse header")
-      | Some res => case res of (vars,clauses) =>
-        (case parse_dimacs_body_arr lno vars fd [] of
-          Inl fail => Inl fail
-        | Inr acc =>
-          if List.length acc = clauses then
-            Inr (vars,(clauses,acc))
-          else
-            Inl (format_dimacs_failure lno "incorrect number of clauses")))
-    else parse_dimacs_toks_arr (lno+1) fd` |> append_prog;
-
-Theorem parse_dimacs_toks_arr_spec:
-  !lines fd fdv fs lno lnov.
-  NUM lno lnov
-  ⇒
-  app (p : 'ffi ffi_proj)
-    ^(fetch_v "parse_dimacs_toks_arr" (get_ml_prog_state()))
-    [lnov; fdv]
-    (STDIO fs * INSTREAM_LINES #"\n" fd fdv lines fs)
-    (POSTv v.
-      & (∃err. SUM_TYPE STRING_TYPE (PAIR_TYPE NUM (PAIR_TYPE NUM (LIST_TYPE (LIST_TYPE INT))))
-      (case parse_dimacs_toks (MAP toks lines) of
-        NONE => INL err
-      | SOME x => INR x) v) *
-      SEP_EXISTS k lines'.
-         STDIO (forwardFD fs fd k) * INSTREAM_LINES #"\n" fd fdv lines' (forwardFD fs fd k))
-Proof
-  Induct
-  \\ simp []
-  \\ rpt strip_tac
-  \\ xcf "parse_dimacs_toks_arr" (get_ml_prog_state ())
-  THEN1 (
-    xlet ‘(POSTv v.
-            SEP_EXISTS k.
-                STDIO (forwardFD fs fd k) *
-                INSTREAM_LINES #"\n" fd fdv [] (forwardFD fs fd k) *
-                &OPTION_TYPE (LIST_TYPE (SUM_TYPE STRING_TYPE INT)) NONE v)’
-    THEN1 (
-      xapp_spec b_inputLineTokens_specialize
-      \\ qexists_tac `emp`
-      \\ qexists_tac ‘[]’
-      \\ qexists_tac ‘fs’
-      \\ qexists_tac ‘fd’ \\ xsimpl \\ fs [])
-    \\ fs [std_preludeTheory.OPTION_TYPE_def] \\ rveq \\ fs []
-    \\ xmatch \\ fs []
-    \\ simp[parse_dimacs_toks_def]
-    \\ xlet_autop
-    \\ xcon \\ xsimpl
-    \\ simp[SUM_TYPE_def]
-    \\ qexists_tac ‘k’ \\ xsimpl
-    \\ qexists_tac `[]` \\ xsimpl
-    \\ metis_tac[])
-  \\ xlet ‘(POSTv v.
-            SEP_EXISTS k.
-                STDIO (forwardFD fs fd k) *
-                INSTREAM_LINES #"\n" fd fdv lines (forwardFD fs fd k) *
-                & OPTION_TYPE (LIST_TYPE (SUM_TYPE STRING_TYPE INT)) (SOME (toks h)) v)’
-    THEN1 (
-      xapp_spec b_inputLineTokens_specialize
-      \\ qexists_tac `emp`
-      \\ qexists_tac ‘h::lines’
-      \\ qexists_tac ‘fs’
-      \\ qexists_tac ‘fd’ \\ xsimpl \\ fs []
-      \\ rw [] \\ qexists_tac ‘x’ \\ xsimpl
-      \\ simp[toks_def])
-  \\ fs [std_preludeTheory.OPTION_TYPE_def] \\ rveq \\ fs []
-  \\ xmatch \\ fs []
-  \\ xlet_autop
-  \\ simp[parse_dimacs_toks_def]
-  \\ reverse IF_CASES_TAC
-  >- (
-    xif >> asm_exists_tac>>xsimpl>>
-    xlet_autop>>
-    xapp>> xsimpl>>
-    asm_exists_tac>> simp[]>>
-    qexists_tac`emp`>>xsimpl>>
-    qexists_tac`forwardFD fs fd k`>>
-    qexists_tac`fd`>>xsimpl>>
-    rw[]>>
-    fs[parse_dimacs_toks_def]>>
-    qexists_tac`k+x`>>
-    simp[GSYM fsFFIPropsTheory.forwardFD_o]>>
-    qexists_tac`x'`>>xsimpl>>
-    metis_tac[])>>
-  xif>> asm_exists_tac>>simp[]>>
-  xlet_autop>>
-  Cases_on`parse_header_line (toks h)`>>fs[OPTION_TYPE_def]
-  >- (
-    xmatch>>
-    xlet_autop>>
-    xcon>>
-    xsimpl>>
-    qexists_tac`k`>> qexists_tac`lines`>>xsimpl>>
-    simp[SUM_TYPE_def]>>
-    metis_tac[])>>
-  xmatch>>
-  Cases_on`x`>>fs[PAIR_TYPE_def]>>
-  xmatch>>
-  xlet_autop>>
-  xlet `(POSTv v.
-      & (∃err. SUM_TYPE STRING_TYPE (LIST_TYPE (LIST_TYPE INT))
-      (case parse_dimacs_body q (FILTER nocomment_line (MAP toks lines)) [] of
-        NONE => INL err
-      | SOME x => INR x) v) *
-      SEP_EXISTS k lines'.
-         STDIO (forwardFD fs fd k) * INSTREAM_LINES #"\n" fd fdv lines' (forwardFD fs fd k))`
-  >- (
-    xapp>>xsimpl>>
-    qexists_tac`emp`>>
-    asm_exists_tac>>simp[]>>
-    asm_exists_tac>>simp[]>>
-    qexists_tac`lines`>>
-    qexists_tac`forwardFD fs fd k`>>
-    qexists_tac`fd`>>xsimpl>>
-    qexists_tac`[]`>>simp[LIST_TYPE_def]>>
-    rw[]>>
-    qexists_tac`k+x`>>
-    simp[GSYM fsFFIPropsTheory.forwardFD_o]>>
-    qexists_tac`x'`>>xsimpl>>
-    metis_tac[])>>
-  pop_assum mp_tac>> TOP_CASE_TAC>>fs[OPTION_TYPE_def]
-  >- (
-    rw[]>>fs[SUM_TYPE_def]>>
-    xmatch>>
-    xcon>>
-    xsimpl>>
-    qexists_tac`k`>>qexists_tac`lines'`>>xsimpl>>
-    metis_tac[])>>
-  strip_tac>>fs[SUM_TYPE_def]>>
-  xmatch>>
-  xlet_autop>>
-  xlet_autop>>
-  drule LENGTH_parse_dimacs_body>>
-  strip_tac>>fs[]>>
-  rw[]>> xif
-  >- (
-    asm_exists_tac>>simp[]>>
-    xlet_autop>>
-    xlet_autop>>
-    xcon>>xsimpl>>
-    simp[SUM_TYPE_def,PAIR_TYPE_def]>>
-    qexists_tac`k`>>qexists_tac`lines'`>>xsimpl)>>
-  asm_exists_tac>>simp[]>>
-  xlet_autop>>
-  xcon>>
-  xsimpl>>
-  qexists_tac`k`>>
-  qexists_tac`lines'`>>
-  simp[SUM_TYPE_def,PAIR_TYPE_def]>>
-  xsimpl>>
-  metis_tac[]
-QED
-
-(* parse_dimacs_toks with simple wrapper *)
-val parse_dimacs_full = (append_prog o process_topdecs) `
-  fun parse_dimacs_full fname =
-  let
-    val fd = TextIO.b_openIn fname
-    val res = parse_ext_dimacs_toks_arr 0 fd
-    val close = TextIO.b_closeIn fd;
-  in
-    res
-  end
-  handle TextIO.BadFileName => Inl (notfound_string fname)`;
-
-Definition get_fml_def:
-  get_fml fs f =
-  if inFS_fname fs f then
-    parse_dimacs_toks (MAP toks (all_lines fs f))
-  else NONE
-End
-
-Theorem parse_dimacs_full_spec:
-  STRING_TYPE f fv ∧
-  validArg f ∧
-  hasFreeFD fs
-  ⇒
-  app (p:'ffi ffi_proj) ^(fetch_v"parse_dimacs_full"(get_ml_prog_state()))
-    [fv]
-    (STDIO fs)
-    (POSTv v.
-    & (∃err. (SUM_TYPE STRING_TYPE (PAIR_TYPE NUM (PAIR_TYPE NUM (LIST_TYPE (LIST_TYPE INT))))
-    (case get_fml fs f of
-      NONE => INL err
-    | SOME x => INR x)) v) * STDIO fs)
-Proof
-  rw[]>>
-  xcf"parse_dimacs_full"(get_ml_prog_state()) >>
-  fs[validArg_def,get_fml_def]>>
-  reverse (Cases_on `STD_streams fs`)
-  >- (fs [TextIOProofTheory.STDIO_def] \\ xpull) >>
-  reverse (Cases_on`consistentFS fs`)
-  >- (fs [STDIO_def,IOFS_def,wfFS_def,consistentFS_def] \\ xpull \\ metis_tac[]) >>
-  reverse (Cases_on `inFS_fname fs f`) >> simp[]
-  >- (
-    xhandle`POSTe ev.
-      &BadFileName_exn ev *
-      &(~inFS_fname fs f) *
-      STDIO fs`
-    >-
-      (xlet_auto_spec (SOME b_openIn_STDIO_spec) \\ xsimpl)
-    >>
-      fs[BadFileName_exn_def]>>
-      xcases>>rw[]>>
-      xlet_auto>>xsimpl>>
-      xcon>>xsimpl>>
-      simp[SUM_TYPE_def]>>metis_tac[])>>
-  qmatch_goalsub_abbrev_tac`$POSTv Qval`>>
-  xhandle`$POSTv Qval` \\ xsimpl >>
-  qunabbrev_tac`Qval`>>
-  xlet_auto_spec (SOME (b_openIn_spec_lines |> Q.GEN`c0` |> Q.SPEC`#"\n"`)) \\ xsimpl >>
-  qmatch_goalsub_abbrev_tac`STDIO fss`>>
-  qmatch_goalsub_abbrev_tac`INSTREAM_LINES _ fdd fddv lines fss`>>
-  xlet`(POSTv v.
-      & (∃err. SUM_TYPE STRING_TYPE (PAIR_TYPE NUM (PAIR_TYPE NUM (LIST_TYPE (LIST_TYPE INT))))
-      (case parse_dimacs_toks (MAP toks lines) of
-        NONE => INL err
-      | SOME x => INR x) v) *
-      SEP_EXISTS k lines'.
-         STDIO (forwardFD fss fdd k) * INSTREAM_LINES #"\n" fdd fddv lines' (forwardFD fss fdd k))`
-  >- (
-    xapp>>xsimpl>>
-    qexists_tac`emp`>>qexists_tac`lines`>>
-    qexists_tac`fss`>>qexists_tac`fdd`>>xsimpl>>
-    rw[]>>
-    qexists_tac`x`>>qexists_tac`x'`>>xsimpl>>
-    metis_tac[])>>
-  xlet `POSTv v. STDIO fs`
-  >- (
-    xapp_spec b_closeIn_spec_lines >>
-    qexists_tac `emp`>>
-    qexists_tac `lines'` >>
-    qexists_tac `forwardFD fss fdd k` >>
-    qexists_tac `fdd` >>
-    qexists_tac `#"\n"` >>
-    conj_tac THEN1
-     (unabbrev_all_tac
-      \\ imp_res_tac fsFFIPropsTheory.nextFD_ltX \\ fs []
-      \\ imp_res_tac fsFFIPropsTheory.STD_streams_nextFD \\ fs []) >>
-    xsimpl>>
-    `validFileFD fdd (forwardFD fss fdd k).infds` by
-      (unabbrev_all_tac>> simp[validFileFD_forwardFD]
-       \\ imp_res_tac fsFFIPropsTheory.nextFD_ltX \\ fs []
-       \\ match_mp_tac validFileFD_nextFD \\ fs []) >>
-    xsimpl >> rw [] >>
-    imp_res_tac (DECIDE ``n<m:num ==> n <= m``) >>
-    imp_res_tac fsFFIPropsTheory.nextFD_leX \\ fs [] >>
-    drule fsFFIPropsTheory.openFileFS_ADELKEY_nextFD >>
-    fs [Abbr`fss`] \\ xsimpl \\ cheat)>>
-  xvar>>
-  xsimpl>>
-  cheat
-QED
-*)
-
 (* parse_dimacs_toks with simple wrapper *)
 val parse_dimacs_full = (append_prog o process_topdecs) `
   fun parse_dimacs_full fname =
@@ -537,7 +157,34 @@ val fill_arr = process_topdecs`
   fun fill_arr arr i ls =
     case ls of [] => arr
     | (v::vs) =>
-      fill_arr (Array.updateResize arr None i (Some (v,3))) (i+1) vs` |> append_prog
+      fill_arr (Array.updateResize arr None i (Some (v,False))) (i+1) vs` |> append_prog
+
+Theorem fill_arr_spec:
+  ∀ls lsv arrv arrls arrlsv i iv.
+  NUM i iv ∧
+  LIST_TYPE a ls lsv ∧
+  LIST_REL (OPTION_TYPE (PAIR_TYPE a BOOL)) arrls arrlsv
+  ⇒
+  app (p:'ffi ffi_proj) ^(fetch_v"fill_arr"(get_ml_prog_state()))
+  [arrv; iv; lsv]
+  (ARRAY arrv arrlsv)
+  (POSTv resv.
+  SEP_EXISTS arrlsv'. ARRAY resv arrlsv' *
+    & LIST_REL (OPTION_TYPE (PAIR_TYPE a BOOL))
+    (FOLDL (λacc (i,v).  update_resize acc NONE (SOME (v,F)) i) arrls (enumerate i ls)) arrlsv')
+Proof
+  Induct>>rw[]>>
+  xcf "fill_arr" (get_ml_prog_state ())>>
+  fs[LIST_TYPE_def,miscTheory.enumerate_def]>>
+  xmatch
+  >- (xvar>>xsimpl)>>
+  rpt xlet_autop >>
+  xlet_auto>>
+  xapp>>xsimpl>>
+  irule LIST_REL_update_resize>>
+  simp[OPTION_TYPE_def,PAIR_TYPE_def]>>
+  EVAL_TAC
+QED
 
 Definition print_result_def:
   (print_result (INL ()) = strlit "s VERIFIED UNSAT\n") ∧
@@ -564,68 +211,6 @@ val check_unsat_2 = (append_prog o process_topdecs) `
       TextIO.print (print_result res)
   end`
 
-(*
-val _ = translate print_lit_def;
-val _ = translate print_clause_def;
-val _ = translate print_xor_def;
-val _ = translate print_header_line_def;
-val _ = translate print_cnf_xor_def;
-
-val check_unsat_1 = (append_prog o process_topdecs) `
-  fun check_unsat_1 f1 =
-  case parse_full f1 of
-    Inl err => TextIO.output TextIO.stdErr err
-  | Inr (mv,(ncl,fml)) => TextIO.print_list (print_cnf_xor fml)`
-
-Definition check_unsat_1_sem_def:
-  check_unsat_1_sem fs f1 err =
-  if inFS_fname fs f1 then
-    (case parse_cnf_xor (all_lines fs f1) of
-      NONE => add_stderr fs err
-    | SOME fml => add_stdout fs (concat (print_cnf_xor fml)))
-  else add_stderr fs err
-End
-
-Theorem check_unsat_1_spec:
-  STRING_TYPE f1 f1v ∧
-  validArg f1 ∧
-  hasFreeFD fs
-  ⇒
-  app (p:'ffi ffi_proj) ^(fetch_v"check_unsat_1"(get_ml_prog_state()))
-    [f1v]
-    (STDIO fs)
-    (POSTv uv. &UNIT_TYPE () uv *
-    SEP_EXISTS err. STDIO (check_unsat_1_sem fs f1 err))
-Proof
-  rw[]>>
-  xcf "check_unsat_1" (get_ml_prog_state ())>>
-  xlet_autop>>
-  simp[check_unsat_1_sem_def]>>
-  TOP_CASE_TAC>>fs[]
-  >- (
-    simp[parse_cnf_xor_def]>>
-    every_case_tac>>fs[SUM_TYPE_def,PAIR_TYPE_def]>>
-    xmatch
-    >- (
-      xapp_spec output_stderr_spec \\ xsimpl>>
-      asm_exists_tac>>xsimpl>>
-      qexists_tac`emp`>>xsimpl>>
-      qexists_tac`fs`>>xsimpl>>
-      rw[]>>qexists_tac`err`>>xsimpl)>>
-    xlet_autop>>
-    xapp_spec print_list_spec>>xsimpl>>
-    asm_exists_tac>>xsimpl>>
-    qexists_tac`emp`>>qexists_tac`fs`>>xsimpl)>>
-  fs[SUM_TYPE_def]>>
-  xmatch>>
-  xapp_spec output_stderr_spec \\ xsimpl>>
-  asm_exists_tac>>xsimpl>>
-  qexists_tac`emp`>>xsimpl>>
-  qexists_tac`fs`>>xsimpl>>
-  rw[]>>qexists_tac`err`>>xsimpl
-QED
-*)
-
 val main = (append_prog o process_topdecs) `
   fun main u =
   case CommandLine.arguments () of
@@ -642,29 +227,25 @@ val b_inputAllTokensFrom_spec_specialize =
   |> Q.GEN `a` |> Q.ISPEC`SUM_TYPE STRING_TYPE INT`
   |> REWRITE_RULE [blanks_v_thm,tokenize_v_thm,blanks_def] ;
 
-(*
 Definition check_unsat_2_sem_def:
   check_unsat_2_sem fs f1 f2 err =
   if inFS_fname fs f1 then
-  (case parse_cnf_xor_toks (MAP toks (all_lines fs f1)) of
+  (case parse_ext_dimacs_toks (MAP toks (all_lines fs f1)) of
     NONE => add_stderr fs err
-  | SOME (mv,ncl,cfml,xfml) =>
-    let cfml = conv_cfml cfml in
+  | SOME (mv,ncl,vars,fml) =>
     if inFS_fname fs f2 then
-      case parse_xlrups (all_lines fs f2) of
-        SOME xlrups =>
-        let cfmlls = enumerate 1 cfml in
+      case parse_scpsteps (all_lines fs f2) of
+        SOME scpsteps =>
+        let pc = mk_pc mv ncl vars in
+        let fmlls = enumerate 1 fml in
         let base = REPLICATE (2*ncl) NONE in
-        let cupd = FOLDL (λacc (i,v). update_resize acc NONE (SOME v) i) base cfmlls in
-        let base = REPLICATE (2*ncl) NONE in
-        let tn = (LN,1) in
+        let cupd = FOLDL (λacc (i,v).
+            update_resize acc NONE (SOME (v,F)) i) base fmlls in
         let bnd = 2*mv+3 in
-          if check_xlrups_unsat_list xfml xlrups cupd base tn
-            0 (REPLICATE bnd w8z)
-          then
-            add_stdout fs (strlit "s VERIFIED UNSAT\n")
-          else
-            add_stderr fs err
+          (case check_scp_final_list scpsteps pc cupd init_sc (REPLICATE bnd w8z) of
+            NONE => add_stderr fs err
+          | SOME res =>
+            add_stdout fs (print_result res))
       | NONE => add_stderr fs err
     else add_stderr fs err)
   else add_stderr fs err
@@ -675,151 +256,6 @@ val err_tac = xapp_spec output_stderr_spec \\ xsimpl>>
     qexists_tac`emp`>>xsimpl>>
     qexists_tac`fs`>>xsimpl>>
     rw[]>>qexists_tac`err`>>xsimpl;
-
-Definition bounded_lit_def:
-  bounded_lit (vars:num) l =
-    case l of
-      Pos v => v ≤ vars
-    | Neg v => v ≤ vars
-End
-
-Theorem parse_lits_aux_bound:
-  ∀vars l acc c.
-  parse_lits_aux vars l acc = SOME c ∧
-  EVERY (bounded_lit vars) acc
-  ⇒
-  EVERY (bounded_lit vars) c
-Proof
-  ho_match_mp_tac parse_lits_aux_ind>>
-  rw[parse_lits_aux_def]>>gvs[AllCaseEqs()]>>
-  first_x_assum match_mp_tac>>
-  rw[bounded_lit_def]
-QED
-
-Theorem parse_clause_bound:
-  parse_clause vars l = SOME c ⇒
-  EVERY (bounded_lit vars) c
-Proof
-  rw[parse_clause_def]>>
-  match_mp_tac parse_lits_aux_bound>>
-  first_x_assum (irule_at Any)>>
-  simp[]
-QED
-
-Theorem parse_line_bound_INL:
-  parse_line vars l = SOME (INL c) ⇒
-  EVERY (bounded_lit vars) c
-Proof
-  rw[parse_line_def]>>
-  gvs[AllCaseEqs()]>>
-  metis_tac[parse_clause_bound]
-QED
-
-Theorem parse_body_bound_cacc:
-  ∀ss vars cacc xacc cacc' xacc'.
-  parse_body vars ss cacc xacc = SOME (cacc',xacc') ∧
-  EVERY (EVERY (bounded_lit vars)) cacc
-  ⇒
-  EVERY (EVERY (bounded_lit vars)) cacc'
-Proof
-  Induct>>rw[parse_body_def]>>
-  gvs[AllCaseEqs()]>>
-  first_x_assum match_mp_tac>>
-  last_x_assum (irule_at Any)>>
-  fs[]>>
-  metis_tac[parse_line_bound_INL]
-QED
-
-Theorem parse_cnf_xor_toks_bound:
-  parse_cnf_xor_toks (MAP toks (all_lines fs f1)) =
-    SOME (vars,ncx,cacc,xacc) ⇒
-  EVERY (EVERY (bounded_lit vars)) cacc
-Proof
-  rw[parse_cnf_xor_toks_def]>>
-  gvs[AllCaseEqs()]>>
-  drule parse_body_bound_cacc>>
-  simp[]
-QED
-
-Theorem LENGTH_FOLDR_update_resize2:
-  ∀ll x.
-  MEM x ll ⇒
-  FST x < LENGTH (FOLDR (λx acc. (λ(i,v). update_resize acc NONE (SOME v) i) x) (REPLICATE n NONE) ll)
-Proof
-  Induct>>simp[FORALL_PROD]>>rw[]>>
-  rw[Once update_resize_def]
-  >- (
-    first_x_assum drule>>
-    simp[])>>
-  first_x_assum drule>>simp[]
-QED
-
-Theorem FOLDL_update_resize_lookup:
-  ∀ls.
-  ALL_DISTINCT (MAP FST ls) ⇒
-  ∀x.
-  x < LENGTH (FOLDL (λacc (i,v). update_resize acc NONE (SOME v) i) (REPLICATE n NONE) ls)
-  ⇒
-  EL x (FOLDL (λacc (i,v). update_resize acc NONE (SOME v) i) (REPLICATE n NONE) ls)
-  =
-  ALOOKUP ls x
-Proof
-  simp[Once (GSYM EVERY_REVERSE), Once (GSYM MAP_REVERSE)]>>
-  simp[FOLDL_FOLDR_REVERSE]>>
-  simp[GSYM alookup_distinct_reverse]>>
-  simp[Once all_distinct_map_fst_rev]>>
-  strip_tac>>
-  qabbrev_tac`ll= REVERSE ls`>>
-  pop_assum kall_tac>>
-  Induct_on`ll`>-
-    simp[EL_REPLICATE]>>
-  simp[FORALL_PROD]>>
-  rw[]>>
-  pop_assum mp_tac>>
-  simp[Once update_resize_def]>>
-  strip_tac>>
-  simp[Once update_resize_def]>>
-  IF_CASES_TAC>>fs[]
-  >-
-    (simp[EL_LUPDATE]>>
-    IF_CASES_TAC>>simp[])>>
-  simp[EL_LUPDATE]>>
-  IF_CASES_TAC >> simp[]>>
-  simp[EL_APPEND_EQN]>>rw[]>>
-  simp[EL_REPLICATE]>>
-  CCONTR_TAC>>fs[]>>
-  Cases_on`ALOOKUP ll x`>>fs[]>>
-  drule ALOOKUP_MEM>>
-  strip_tac>>
-  drule LENGTH_FOLDR_update_resize2>>
-  simp[]>>
-  metis_tac[]
-QED
-
-Theorem bounded_cfml_FOLDL_enumerate:
-  EVERY (EVERY (bounded_lit vars)) ls ∧
-  v > 2 * vars ⇒
-  bounded_cfml v
-    (FOLDL (λacc (i,v). update_resize acc NONE (SOME v) i)
-     (REPLICATE n NONE) (enumerate k (conv_cfml ls)))
-Proof
-  rw[bounded_cfml_def]>>
-  simp[Once EVERY_EL]>>rw[]>>
-  `ALL_DISTINCT (MAP FST (enumerate k (conv_cfml ls)))` by
-    metis_tac[ALL_DISTINCT_MAP_FST_enumerate]>>
-  TOP_CASE_TAC>>simp[]>>
-  drule FOLDL_update_resize_lookup>>
-  disch_then drule>>
-  disch_then (SUBST_ALL_TAC)>>
-  drule ALOOKUP_MEM>>
-  strip_tac>> drule MEM_enumerate_IMP>>
-  fs[EVERY_MEM]>>
-  simp[conv_cfml_def,MEM_MAP,PULL_EXISTS,EVERY_MEM]>>
-  rw[]>>
-  first_x_assum drule_all>>
-  simp[bounded_lit_def]>>every_case_tac>>
-  rw[conv_lit_def,index_def]
-QED
 
 Theorem check_unsat_2_spec:
   STRING_TYPE f1 f1v ∧ validArg f1 ∧
@@ -838,108 +274,92 @@ Proof
   simp[check_unsat_2_sem_def]>>
   reverse TOP_CASE_TAC>>fs[]
   >- (
-    fs[SUM_TYPE_def]>>xmatch>>
+    gvs[get_prob_def,SUM_TYPE_def]>>xmatch>>
     err_tac)>>
+  gvs[get_prob_def,SUM_TYPE_def]>>
   TOP_CASE_TAC>> fs[SUM_TYPE_def]
   >- (xmatch>> err_tac)>>
   PairCases_on`x`>>fs[SUM_TYPE_def,PAIR_TYPE_def]>>
   xmatch>>
-  rename1`_ = SOME (_,_,cfml,xfml)`>>
+  rename1`_ = SOME (nv,nc,vars,fml)`>>
   xlet_autop>>
   xlet`POSTv v. &NUM 1 v * STDIO fs` >- (xlit>>xsimpl)>>
   rw[]>>
   (drule_at (Pos (hd o tl))) fill_arr_spec>>
   (* help instantiate fill_arr_spec *)
-  `LIST_REL (OPTION_TYPE (LIST_TYPE INT)) (REPLICATE (2 * x1) NONE)
-        (REPLICATE (2 * x1) (Conv (SOME (TypeStamp "None" 2)) []))` by
+  `LIST_REL (OPTION_TYPE (PAIR_TYPE (LIST_TYPE INT) BOOL)) (REPLICATE (2 * nc) NONE)
+        (REPLICATE (2 * nc) (Conv (SOME (TypeStamp "None" 2)) []))` by
     simp[LIST_REL_REPLICATE_same,OPTION_TYPE_def]>>
   qpat_x_assum`NUM 1 _` assume_tac>>
   disch_then drule>>
   disch_then drule>>
   rw[]>>rpt xlet_autop>>
-  (*
-  fs[PAIR_TYPE_def]>>
-  xmatch>>
-  rpt xlet_autop>>
-  (drule_at (Pos (hd o tl))) fill_arr_spec>>
-  (* help instantiate fill_arr_spec *)
-  `LIST_REL (OPTION_TYPE STRING_TYPE) (REPLICATE (2 * x1) NONE)
-        (REPLICATE (2 * x1) (Conv (SOME (TypeStamp "None" 2)) []))` by
-    simp[LIST_REL_REPLICATE_same,OPTION_TYPE_def]>>
-  qpat_x_assum`NUM 1 _` assume_tac>>
-  disch_then drule>>
-  disch_then drule>>
-  rw[]>>
-  rpt xlet_autop>> *)
-  simp[check_xlrups_unsat_list_def]>>
-  qmatch_goalsub_abbrev_tac`check_xlrups_list _ _ a b c d e`>>
-  xlet`POSTv v.
+  simp[check_scp_final_list_def]>>
+  qmatch_goalsub_abbrev_tac`check_scpsteps_list _ a b c d`>>
+  xlet`(POSTv v.
     STDIO fs *
     SEP_EXISTS err.
-     &SUM_TYPE STRING_TYPE BOOL
+      &(SUM_TYPE STRING_TYPE res_TYPE)
       (if inFS_fname fs f2 then
-         (case parse_xlrups (all_lines fs f2) of
-            NONE => INL err
-          | SOME xlrups =>
-            (case check_xlrups_list xfml xlrups a b c d e of
+        (case parse_scpsteps (all_lines fs f2) of
+         SOME scpsteps =>
+           (case check_scp_final_list scpsteps a b c d of
              NONE => INL err
-           | SOME (cfml', xfml') =>
-           INR (contains_emp_list cfml')))
-       else INL err) v`
+           | SOME res => INR res)
+        | NONE => INL err)
+      else
+        INL err
+      ) v)`
   >- (
     xapp_spec (GEN_ALL check_unsat'_spec)>>
     xsimpl>>
     asm_exists_tac>>simp[]>>
     fs[FILENAME_def,validArg_def]>>
     asm_exists_tac>>simp[]>>
-    asm_exists_tac>>simp[]>>
     first_x_assum (irule_at Any)>>
     first_x_assum (irule_at Any)>>
-    qexists_tac`REPLICATE (2 * x1) NONE`>>
-    qexists_tac`(LN,1)`>>
+    first_x_assum (irule_at Any)>>
+    first_x_assum (irule_at Any)>>
+    first_x_assum (irule_at Any)>>
+    qexists_tac`init_sc`>>
     xsimpl>>
-    reverse CONJ_TAC >- (
-      CONJ_TAC >-
-        metis_tac[LIST_REL_REPLICATE_same,OPTION_TYPE_def]>>
-      CONJ_TAC >- (
-        simp[PAIR_TYPE_def,Abbr`c`]>>
-        EVAL_TAC)>>
-      rw[]>>metis_tac[])>>
-    (* bounded_cfml *)
-    drule parse_cnf_xor_toks_bound>>
-    fs[Abbr`a`]>>
-    strip_tac>>
-    drule bounded_cfml_FOLDL_enumerate>>
-    disch_then match_mp_tac>>
-    simp[])>>
+    rw[]
+    >-
+      gvs[Abbr`c`,fetch "-""init_sc_v_thm"]
+    >- cheat
+      (*
+      drule parse_cnf_xor_toks_bound>>
+      fs[Abbr`a`]>>
+      strip_tac>>
+      drule bounded_cfml_FOLDL_enumerate>>
+      disch_then match_mp_tac>>
+      simp[] *)
+    >- metis_tac[]
+    >- metis_tac[])>>
   reverse TOP_CASE_TAC>>simp[]
   >- (fs[SUM_TYPE_def]>>xmatch>>err_tac)>>
   TOP_CASE_TAC>>fs[SUM_TYPE_def]
   >- (xmatch>>err_tac)>>
-  Cases_on`check_xlrups_list xfml x a b c d e`>>fs[SUM_TYPE_def]
-  >- (xmatch>>err_tac)>>
-  Cases_on`x'`>>fs[]>>
-  fs[SUM_TYPE_def]>>
-  xmatch>>
-  xif
+  gvs[check_scp_final_list_def]>>
+  Cases_on`check_scpsteps_list x a b c d`>>fs[SUM_TYPE_def]
   >- (
-    xapp_spec print_spec >> xsimpl
-    \\ qexists_tac`emp`
-    \\ qexists_tac`fs`>>xsimpl)
-  >- (
-    gs[GSYM quantHeuristicsTheory.IS_SOME_EQ_NOT_NONE,IS_SOME_EXISTS,OPTION_TYPE_def]>>
-    xapp_spec output_stderr_spec \\ xsimpl>>
-    qexists_tac`emp`>>xsimpl>>
-    qexists_tac`fs`>>xsimpl>>
-    rw[]>>
-    qmatch_goalsub_abbrev_tac`_ _ err`>>
-    qexists_tac`err`>>xsimpl)
+    xmatch>>
+    err_tac)>>
+  PairCases_on`x'`>>fs[]>>
+  rename1`check_final_list a xx yy`>>
+  Cases_on`check_final_list a xx yy`>>fs[SUM_TYPE_def]>>
+  xmatch
+  >- err_tac>>
+  xlet_autop>>
+  xapp_spec print_spec >> xsimpl
+  \\ qexists_tac`emp`
+  \\ asm_exists_tac
+  \\ qexists_tac`fs`>>xsimpl
 QED
 
 Definition main_sem_def:
   main_sem cl fs err =
   case TL cl of
-  | [f1] => check_unsat_1_sem fs f1 err
   | [f1;f2] => check_unsat_2_sem fs f1 f2 err
   | _ => add_stderr fs err
 End
@@ -968,12 +388,11 @@ Proof
     qexists_tac`fs`>>xsimpl>>
     rw[]>>qexists_tac`usage_string`>>xsimpl)
   >- (
-    xapp>>xsimpl>>
+    xapp_spec output_stderr_spec \\ xsimpl>>
     qexists_tac`COMMANDLINE cl`>>xsimpl>>
-    qexists_tac`fs`>>qexists_tac`h'`>>xsimpl>>
-    fs[wfcl_def,Abbr`cl`]>>
-    rw[]>>
-    qexists_tac`x`>>xsimpl)
+    qexists_tac `usage_string` >> simp [theorem "usage_string_v_thm"] >>
+    qexists_tac`fs`>>xsimpl>>
+    rw[]>>qexists_tac`usage_string`>>xsimpl)
   >- (
     xapp>>xsimpl>>
     qexists_tac`COMMANDLINE cl`>>xsimpl>>
@@ -990,27 +409,10 @@ Proof
     qexists_tac`fs`>>xsimpl>>
     rw[]>>qexists_tac`usage_string`>>xsimpl)
 QED
-*)
-
-Definition main_sem_def:
-  main_sem cl fs err = fs
-End
-
-Theorem main_spec:
-   hasFreeFD fs
-   ⇒
-   app (p:'ffi ffi_proj) ^(fetch_v"main"(get_ml_prog_state()))
-     [Conv NONE []]
-     (COMMANDLINE cl * STDIO fs)
-     (POSTv uv. &UNIT_TYPE () uv *
-     COMMANDLINE cl * SEP_EXISTS err. STDIO (main_sem cl fs err))
-Proof
-  cheat
-QED
 
 Theorem main_whole_prog_spec2:
    hasFreeFD fs ⇒
-   whole_prog_spec2 main_v cl fs NONE (λfs'. ∃err. fs' = main_sem cl fs err)
+   whole_prog_spec2 main_v_0 cl fs NONE (λfs'. ∃err. fs' = main_sem cl fs err)
 Proof
   rw[basis_ffiTheory.whole_prog_spec2_def]
   \\ match_mp_tac (MP_CANON (DISCH_ALL (MATCH_MP app_wgframe (UNDISCH main_spec))))
@@ -1019,7 +421,9 @@ Proof
   \\ qexists_tac`main_sem cl fs x`
   \\ qexists_tac`x`
   \\ xsimpl
-  \\ cheat
+  \\ simp[main_sem_def,check_unsat_2_sem_def]
+  \\ every_case_tac
+  \\ simp[GSYM add_stdo_with_numchars,with_same_numchars]
 QED
 
 local
